theories/equivalence/LanguagesEquivalence.v
@@ -1,14 +1,18 @@
 From Triq Require NatLang.
-From Triq Require NatLangProperties.
 From Triq Require StringLang.
+
+From Triq Require NatLangProperties.
 From Triq Require StringLangProperties.
+
 From Triq Require Import LanguagesCommon.
-From Triq Require Import LanguagesUtils.
 From Triq Require Import StringMacros.
+
+From Triq Require Import NatUtils.
+From Triq Require Import StringUtils.
+From Triq Require Import LanguagesUtils.
 
 From Stdlib Require Import Nat.
 From Stdlib Require Import List.
-From Stdlib Require Extraction.
 From Stdlib Require Import Lia.
 
 Import ListNotations.
@@ -35,17 +39,13 @@ fold_left
   (firstn n p_nat)
 0.
 
-
 Definition equiv_pos 
 (p_nat : NatLang.program) (n : nat)
 (p_str : StringLang.program ) (n' : nat) (max_char : nat) :=
 n' = get_equiv_simulated_position p_nat n max_char.
 
 
-(* TODO: max_z_nat *)
-
-Definition max_z_nat (p : NatLang.program) := 0.
-
+(** Teorema Principal *)
 Theorem nat_implies_string :
   forall (p_nat : NatLang.program)
          (initial_state_nat : NatLang.state)
@@ -68,11 +68,9 @@ Theorem nat_implies_string :
 
   state_equiv state_nat state_str max_char /\
   equiv_pos p_nat line_nat p_str line_str max_char /\
-  (* Posso obter isso de state_equiv, mas é mais fácil carregar a informação como
-    invariante *)
-  (* preciso adicionar state_over 1 do state_str *)
   state_str (Z (max_z_nat p_nat + 1)) = [] /\
   state_str (Z (max_z_nat p_nat + 2)) = [] /\
   StringLang.state_over state_str max_char.
+
 Proof.
-Admitted.
+Admitted. 
