theories/equivalence/NatUtils.v
@@ -1,0 +1,21 @@
+From Triq Require NatLang.
+From Triq Require Import LanguagesCommon.
+
+From Stdlib Require Import Nat.
+From Stdlib Require Import List.
+From Stdlib Require Extraction.
+From Stdlib Require Import Lia.
+Import ListNotations.
+
+(** ** Obtendo a Maior Variável Z em p_nat *)
+
+Fixpoint max_z_nat (l : NatLang.program) : nat :=
+    match l with
+    | [] => 0
+    | NatLang.Instr opt_lbl (NatLang.INCR (Z n))  :: t 
+    | NatLang.Instr opt_lbl (NatLang.DECR (Z n))  :: t 
+    | NatLang.Instr opt_lbl (NatLang.IF_GOTO (Z n) _ )  :: t  =>
+      Nat.max n (max_z_nat t) 
+    | _ :: t => max_z_nat t
+    end.
+
