theories/equivalence/StringUtils.v
@@ -1,0 +1,7 @@
+From Triq Require StringLang.
+From Triq Require Import LanguagesCommon.
+
+From Stdlib Require Import Nat.
+From Stdlib Require Import List.
+From Stdlib Require Import Lia.
+Import ListNotations.
